\setchapterpreamble[u]{\margintoc}
\chapter{3-Dimensional Space}


We've been working with harmonic oscilators and gravitational potentials but there are other interesting potentials that we are going to mention here.

\begin{itemize}
  \item Electric Potential $V(r) = \frac{\alpha}{r}$, $\alpha>0$
  \item Confining Potential $V(r) = k r$
  \item Higgs Potential $V(r) = \frac{\alpha}{r} e^{-mr}$
\end{itemize}

\marginnote[1cm]{There are others like: Reed Potential, Cornell Potential,...}

\section{Angular Momentum in 3 Dimensions}

We can also have potentials that doesn't come from central forces. In those cases we have to look carefully at the angular momentum.

\begin{equation}
  \vec{L} = \vec{r} \times \vec{p}
\end{equation}

\begin{equation}
  \begin{array}{c}
    L_x = y p_z - z p_y\\
    L_y = z p_x - x p_z\\
    L_z = x p_y - y p_x
  \end{array}
\end{equation}

Using our knowledge from equation 2.4 we can say,

\begin{equation}
  \begin{array}{c}
    L_x = -i \hbar (y \frac{\partial}{\partial z} - z \frac{\partial}{\partial y})\\
    L_y = -i \hbar (z \frac{\partial}{\partial x} - x \frac{\partial}{\partial z})\\
    L_z = -i \hbar (x \frac{\partial}{\partial y} - y \frac{\partial}{\partial x})
  \end{array}
\end{equation}

This three components of the angular momentum and the angular momentum itself are hermitian operators. We want to see how they commute between them.

\begin{equation}
  \begin{array}{c}
  (L_xL_y) \psi = -\hbar^2 (y \frac{\partial}{\partial z} - z \frac{\partial}{\partial y})(z \frac{\partial}{\partial x} - x \frac{\partial}{\partial z}) \psi =
  \\

  \\
  = -\hbar^2 \left[y\left(\frac{\partial \psi}{\partial x}+z\frac{\partial^2\psi}{\partial x \partial z}\right)-yx\frac{\partial^2 \psi}{\partial z^2}-z^2 \frac{\partial^2 \psi}{\partial x \partial y}-zx\frac{\partial^2 \psi}{\partial y \partial z}\right] (a)
  \\

  \\
  (L_y L_x) \psi = -\hbar^2 (z \frac{\partial}{\partial x} - x \frac{\partial}{\partial z})(y \frac{\partial}{\partial z} - z \frac{\partial}{\partial y}) \psi =
  \\

  \\
  = -\hbar^2 \left[zy\frac{\partial^2\psi}{\partial x\partial z}-xy\frac{\partial^2\psi}{\partial z^2}-z^2\frac{\partial^2 \psi}{\partial x \partial y}+x\frac{\partial \psi}{\partial y}+xz\frac{\partial^2 \psi}{\partial z \partial y}\right] (b)
  \\

  \\
  (a)-(b) = [L_x,L_y] =i\hbar L_z
  \end{array}
\end{equation}

In the same way it can be prooved that:

\begin{equation}
  \begin{array}{c}
  [L_y,L_z] =i\hbar L_x
  \\

  \\
  [L_z,L_x] =i\hbar L_y
  \end{array}
\end{equation}

These 3 operators are closed under conmmutation, wich means that the conmmutation of any two of them give us the third one.

We our going to use the Levi-Civita epsilon to write the angular momentum in a more compact way.

\marginnote[1cm]{Levi-Civita epsilon has a lot of application in linear algebra. For example it can be used to determine the determinant of a matrix.}

\begin{equation}
  \begin{array}{c}
    [L_i,L_j] = i\hbar \epsilon_{ijk} L_k
  \end{array}
\end{equation}

Now using the properties from 6.22 we want to calculate the conmmutation between $L_i$ and $L_i^2$.

\begin{equation}
  \begin{array}{c}
    [L_i,L_i^2] = [L_i,L_i]L_i + L_i[L_i,L_i] = 0
    \\

    \\
    \left[ L_i,L_j^2 \right] = \left[L_i,L_j\right]L_j + L_j[L_i,L_j] = i \hbar \left(L_k L_j \right) + i \hbar \left( L_j L_k \right) = i \hbar (L_k L_j + L_j L_k)
    \\

    \\
    \left[L_i,L_k^2\right] = [L_i,L_k]L_k + L_k[L_i,L_k] = -i\hbar\left(L_j L_k\right)-i\hbar\left(L_k L_j\right) = -i\hbar(L_k L_j + L_j L_k)
    \\

    \\
    \left[L_i,L_i^2 +L_j^2+L_k^2\right] = [L_i, L] = 0
  \end{array}
\end{equation}

This means that the angular momentum and the square of the angular momentum commute. We can simultaneously diagonalize them because they commute, so a base wher both are diagonalizable can be found.

\begin{equation}
  \label{9.8}
  \begin{array}{c}
    L^2 \ket{l,m} = \hbar^2 l^2 \ket{l,m}
    \\

    \\
    L_3 \ket{l,m} = \hbar m \ket{l,m}
  \end{array}
\end{equation}

We choose this notation for the eigenvalues to make the connection with the eigenvalues. Also we choose the notation 1,2,3 instead of x,y,z. These changes are just for convenience.

In general terms:

\begin{equation}
  \begin{array}{c}
    \left[L^2,L_c\right] = \left[\sum_{n=1}^{3}L_a^2,L_c\right] = \sum_{n=1}^{3}\left[L_a L_a ,L_c\right] =
    \\

    \\
    = \sum_{n=1}^{3} \left(L_a[L_a,L_c] + [L_a,L_c] L_a\right) =
    \\

    \\
    = i\hbar \sum_{a,b=1}^{3} \epsilon_{acb} L_a L_b + i\hbar \sum_{a,b=1}^{3} \epsilon_{acb} L_b L_a =
    \\

    \\
    i\hbar \left(\sum_{a,b=1}^{3} \epsilon_{acb} \epsilon_{bca}\right) L_a L_b = 0
  \end{array}
\end{equation}

\marginnote[-2cm]{We can use the Levi-Civita epsilon to change the order of the indices.}

Going back to equation \ref{9.8} we can say

\begin{equation}\label{9.10}
  \begin{array}{c}
    \bra{l,m}L_a^2\ket{l,m} = (\bra{l,m}L_1)(L_a\ket{l,m}) = (L_a\ket{l,m})^\dagger(L_a\ket{l,m})  \geq 0
    \\

    \\
    \bra{l,m} L_1^2 + L_2^2 \ket{l,m} \geq 0
    \\

    \\
    \bra{l,m} L_1^2 + L_2^2 + L_3^2 - L_3^2 \ket{l,m} \geq 0
    \\

    \\
    \bra{l,m} L^2\ket{l,m} - \bra{l,m} L_3^2 \ket{l,m} \geq 0
    \\

    \\
    \hbar^2 l^2 \braket{l,m}{l,m} - \hbar^2 m^2 \braket{l,m}{l,m} \geq 0
    \\

    \\
    \hbar^2 (l^2 - m^2) \geq 0
    \\

    \\
    l^2 \geq m^2
  \end{array}
\end{equation}

This result means that the proyectionof the angular momentum in the z direction is less or equal to the total angular momentum, as one would expected.

We want to create new operators $L_+$ and $L_-$ that are going to be useful to us.

\begin{equation}
  \begin{array}{c}
    L_+ = L_1 + i L_2
    \\

    \\
    L_- = L_1 - i L_2
  \end{array}
\end{equation}

With the next properties:

\begin{equation}
  \begin{array}{c}
    L_+^\dagger = L_-
    \\

    \\
    L_-^\dagger = L_+
  \end{array}
\end{equation}

As every time, when we have a new operator we want to know it commutes with the rest.

\begin{equation}
  \begin{array}{c}
    \left[L_3, L_+\right] = \left[L_3,L_1\right] + i \left[L_3,L_2\right] = i\hbar L_2 - i i\hbar L_1 = \hbar L_1 + i \hbar L_2 = \hbar L_+
    \\

    \\
    \left[L_3,L_-\right] = \left[L_3,L_1\right] - i \left[L_3,L_2\right] = i\hbar L_2 + i i\hbar L_1 = -\hbar L_1 + i \hbar L_2 = - \hbar L_-
    \\

    \\
    \left[L_+,L_-\right] = \left[L_1 +i L_2, L_1 - iL_2\right] = \left[L_1,L_1\right] + \left[L_2,L_2\right] - i\left[L_1,L_2\right] + i\left[L_2,L_1\right] = 2\hbar L_3
    \\

    \\
    \left[L^2,L_+\right] = \left[L^2,L_1\right] + i \left[L^2,L_2\right] = 0
    \\

    \\
    \left[L^2,L_-\right] = \left[L^2,L_1\right] - i \left[L^2,L_2\right] = 0
  \end{array}
\end{equation}

With this new operators we can get the next eigenvectors for m without changing l.

\begin{equation}
  \begin{array}{c}
    L^2 (L+\ket{l,m}) = L_+ L^2 \ket{l,m} = L_+ \hbar^2 l^2 \ket{l,m} = \hbar^2 l^2 (L_+ \ket{l,m})
  \end{array}
\end{equation}

This means that $L_+\ket{l,m}$ is an eigenvector of $L^2$ with the same eigenvalue $\hbar^2 l^2$.

\begin{equation}
  \begin{array}{c}
  L_3(L_+\ket{l,m}) = (\hbar L_+ + L_+ L_3)\ket{l,m} = \hbar(m+1)(L_+\ket{l,m})
  \end{array}
\end{equation}

This implies that $L_+\ket{l,m}$ is an eigenvector of $L_3$ with eigenvalue $\hbar(m+1)$, i.e, $L_+\ket{l,m} \propto \ket{l,m+1}$. We can do the same for $L_-$.

\begin{equation}
  \begin{array}{c}
    L^2(L_-\ket{l,m}) = L_-\hbar^2 l^2 \ket{l,m} = \hbar^2 l^2 (L_-\ket{l,m})
    \\

    \\
    L_3(L_-\ket{l,m}) = (-\hbar L_- + L_- L_3)\ket{l,m} = \hbar(m-1)(L_-\ket{l,m})
  \end{array}
\end{equation}

This implies that $L_-\ket{l,m}$ is an eigenvector of $L^2$ with eigenvalue $\hbar^2 l^2$ and of $L_3$ with eigenvalue $\hbar(m-1)$, i.e, $L_-\ket{l,m} \propto \ket{l,m-1}$.

We can use $L_+$ and $L_-$ to get all the eigenvalues of $L_3$, but there is a limit because for a fixed l, m can only take values from -l to l as we proved in \ref{9.10}. This can only happen if the next eigenvalue is 0.

\begin{equation}
  \begin{array}{c}
    L_+\ket{l,m_{max}} = 0
    \\

    \\
    L_-\ket{l,m_{min}} = 0
  \end{array}
\end{equation}

We are going to solve for the maximum values of m multiplying by $L_-$.

\begin{equation}
  \begin{array}{c}
    L_- L_+ \ket{l,m_{max}} = 0
    \\

    \\
    (L_1-iL_2)(L_1+iL_2)\ket{l,m_{max}} = 0
    \\

    \\
    [L_1^2+L_2^2 + i(L_1L_2-L_2L_1)]\ket{l,m_{max}} = 0
    \\

    \\
    [L^2 - L_3^2 - \hbar L_3]\ket{l,m_{max}} = 0
    \\

    \\
    (\hbar^2 l^2 - \hbar^2 m_{max}^2 - \hbar^2 m_{max})\ket{l,m_{max}} = 0
    \\

    \\
    \hbar^2 l^2 - \hbar^2 m_{max}^2 - \hbar^2 m_{max} = 0
    \\

    \\
    l^2 = m_{max}^2 + m_{max}
  \end{array}
\end{equation}

Which implies than the maximum m is less than l, this can only happen because $L^2$ and $L_3$ are operators. We can do the same for the minimum value of m.

\begin{equation}
  \begin{array}{c}
    L_+ L_- \ket{l,m_min} = 0
    \\

    \\
    (L_1+iL_2)(L_1-iL_2)\ket{l,m_min} = 0
    \\

    \\
    [L_1^2+L_2^2 - i(L_1L_2-L_2L_1)]\ket{l,m_min} = 0
    \\

    \\
    [L^2 - L_3^2 + \hbar L_3]\ket{l,m_min} = 0
    \\

    \\
    (\hbar^2 l^2 - \hbar^2 m_{min}^2 + \hbar^2 m_{min})\ket{l,m_{min}} = 0
    \\

    \\
    \hbar^2 l^2 - \hbar^2 m_{min}^2 + \hbar^2 m_{min} = 0
    \\

    \\
    l^2 = m_{min}^2 - m_{min}
  \end{array}
\end{equation}

If we compare the limits of m we end up with the next result.

\begin{equation}
  \begin{array}{c}
    m^2_{max} + m_{max} = m^2_{min} - m_{min}
  \end{array}
\end{equation}

This expresion have two solutions:

\begin{equation}
  \begin{array}{c}
    m_{max} = m_{min} - 1
    \\

    \\
    m_{max} = - m_{min}
  \end{array}
\end{equation}

The first solution can be discarted because it would imply that $m_{max}$ is less than $m_{min}$. The second solution is the real one. We know that m increases or decreases by a factor of 1, so we can say that:

\begin{equation}
  \begin{array}{c}
    m_{max} = m_{min} + I
  \end{array}
\end{equation}

Where I is an non-negative integer. If we used what we know about the limits of m we can say that:

\begin{equation}
  \begin{array}{c}
    m_{max} = - m_{max} + I
    \\

    \\
    m_{max} = \frac{I}{2}
  \end{array}
\end{equation}

This means that $L_z$ is quantized, i. e., only some proyections of the angular momentum in the z axis are allowed. We are going to start labeling the eigenfunctions as $\ket{j,m}$ where j is defined by:

\begin{equation}
  \begin{array}{c}
    j = m_{max}
    \\

    \\
    l^2 = j(j+1)
  \end{array}
\end{equation}

Where j can be the natural numbers or half of them, i.e., j = 0, 1/2, 1, 3/2... Now our eigenfunctions follow:

\begin{equation}
  \begin{array}{c}
    L^2 \ket{j,m} = \hbar^2 j(j+1) \ket{j,m}
    \\

    \\
    L_3 \ket{j,m} = \hbar m \ket{j,m}
  \end{array}
\end{equation}

For m = j, j-1, j-2,..., -j. The j,m pair make a completeset of (orthogonal) eigenvectors. Following what we know from \ref{6.29}:

\begin{equation}
  \begin{array}{c}
    \braket{j_1,m_1}{j_1,m_2} = 0 \text{ if } m_1 \neq m_2
    \\

    \\
    \braket{j_1,m_1}{j_2,m_1} = 0 \text{ if } j_1 \neq j_2
  \end{array}
\end{equation}

We also set the normalization condition:

\begin{equation}
  \begin{array}{c}
    \braket{j,m}{j,m} = 1
  \end{array}
\end{equation}

From now we will move on to what an experimentalist will measure.

\section{Angular Momentum as a vector operator}

We can interpret the angular momentum as:

\begin{equation}
  \begin{array}{c}
    \vec{L} = L_1 \hat{i} + L_2 \hat{j} + L_3 \hat{k}
  \end{array}
\end{equation}

In a classical way we know that the angular mometum is conserved, so we can say that all the angular momentum is in one direction.

\begin{equation}
  \begin{array}{c}
    \vec{L} x \vec{L} = (L_2 L_3 - L_3L_2)\hat{i} + (L_3L_1 - L_1L_3)\hat{j} + (L_1L_2 - L_2L_1)\hat{k}
  \end{array}
\end{equation}

In classical mechanics that product is 0 because the components are numbers but in a quantum way they are operators that doesn't commute, in this case the cross product is:

\begin{equation}
  \begin{array}{c}
    \vec{L} x \vec{L} = i\hbar \vec{L}
  \end{array}
\end{equation}

This is the operator equation. On an experiment we can measure the angular momentum of the electron in hydrogen. Assume it is in one state $\psi$.

\begin{equation}
  \begin{array}{c}
    \int_{-\infty}^{\infty} dxdydz \psi^{\star}(x,y,z) O \psi(x,y,z) = \text{ Measurement of O}
  \end{array}
\end{equation}

We are going to make a distintion between the angular momentum $\vec{L}$, and the measured angular momentum, $\vec{l}$.

\begin{equation}
  \begin{array}{c}
    \vec{l} = \bra{s}\vec{L}\ket{s}
    \\

    \\
    \vec{l} = \bra{s}L_1\ket{s}\hat{i} + \bra{s}L_2\ket{s}\hat{j} + \bra{s}L_3\ket{s}\hat{k}
  \end{array}
\end{equation}

With the next properties:

\begin{equation}
  \begin{array}{c}
    \vec{l} x \vec{l} = 0
    \\

    \\
    \vec{l} \cdot \vec{l} = (\bra{s}L_1\ket{s})^2 + (\bra{s}L_2\ket{s})^2 + (\bra{s}L_3\ket{s})^2 \geq 0
  \end{array}
\end{equation}

We want to know the value of this dot product.

\begin{equation}
  \begin{array}{c}
    \bra{j,m}L_3\ket{j,m} = \hbar m \braket{j,m} = \hbar m
    \\

    \\
    \bra{j,m}L_3^2\ket{j,m} = \hbar^2 m^2 = (\bra{j,m}L_3\ket{j,m})^2
    \\

    \\
    \bra{j,m}L^2\ket{j,m} = \hbar^2 j(j+1)
    \\

    \\
    \bra{j,m}L_1^2 + L_2^2\ket{j,m} = \hbar^2 ( j(j+1) - m^2 )
  \end{array}
\end{equation}

To get the value of $\bra{j,m}L_1\ket{j,m}$ we have to use the definition of $L_+$ and $L_-$.

\begin{equation}
  \begin{array}{c}
    \bra{j,m}L_1\ket{j,m} = \bra{j,m}L_+\ket{j,m} + \bra{j,m}iL_-\ket{j,m} =
    \\

    \\
    = N_+ \braket{j,m}{j,m+1} + N_- \braket{j,m}{j,m-1} = 0
  \end{array}
\end{equation}

The same argument can be done for $L_2$. Because of this we can say that:

\begin{equation}\left\{
  \begin{array}{c}
    l_1 = 0
    \\

    \\
    l_2 = 0
    \\

    \\
    l_3 = \hbar m
    \\

    \\
    l^2 = ?
  \end{array}\right.
\end{equation}

We have two definitions if we consider $l^2$ as the measure of $L^2$ is going to be $l^2$ = $\hbar^2 j(j+1)$, but if we consider $l^2$ as the square of the measure L we get $\hbar^2 m^2$. This is exactly the same as talking about the square of the mean or taking about the variance, so we are familiarize with this concepts from chapter 2.

We said before that the operators $L_+$ and $L_-$ are proportional to the next or the previous eigenfunctions. Now we want to find the exact value of the proportionality constant.

\begin{equation}
  \begin{array}{c}
    \L_+ \ket{j,m} = n_{+,j,m} \ket{j,m+1}
    \\

    \\
    L_- \ket{j,m} = n_{-,j,m} \ket{j,m-1}
    \\

    \\
    \braket{j_1,m_1}{j_2,m_2} = \delta_{j_1,j_2}\delta_{m_1,m_2}
  \end{array}
\end{equation}

We can always find real positive values for both $n_+$ and $n_-$. We want them to be like this because we are going to take the conjugate of the expresion above.

\begin{equation}
  \begin{array}{c}
    \bra{j,m}L_- = n_{+,j,m} \bra{j,m+1}
    \\

    \\
    (\bra{j,m}L_-)(L_+\ket{j,m}) = n_{+,j,m}^2  \braket{j,m+1}{j,m+1}
    \\

    \\
    \bra{j,m}(L_1-iL_2)(L_1+iL_2)\ket{j,m} = n_{+,j,m}^2
    \\

    \\
    \bra{j,m}L_1^2+L_2^2-\hbar L_3\ket{j,m} = n_{+,j,m}^2
    \\

    \\
    \hbar^2 j(j+1) - \hbar^2 m^2 - \hbar^2 m \braket{j,m}{j,m} = n_{+,j,m}^2
    \\

    \\
    \hbar^2 [j(j+1) - m(m+1)] = n_{+,j,m}^2
  \end{array}
\end{equation}

We have finally reach the value of $n_{+,j,m}$. We can write now:

\begin{equation}
  \begin{array}{c}
    L_+ \ket{j,m} = \hbar \sqrt{j(j+1) - m(m+1)} \ket{j,m+1}
  \end{array}
\end{equation}

It is easy to prove from this that $L_+\ket{j,j} = 0$, as we wanted. We can do the same for $L_-$.

\begin{equation}
  \begin{array}{c}
    \bra{j,m}L_+ = n_{-,j,m} \bra{j,m-1}
    \\

    \\
    (\bra{j,m}L_+)(L_-\ket{j,m}) = n_{-,j,m}^2  \braket{j,m-1}{j,m-1}
    \\

    \\
    \bra{j,m}(L_1+iL_2)(L_1-iL_2)\ket{j,m} = n_{-,j,m}^2
    \\

    \\
    \bra{j,m}L_1^2+L_2^2+\hbar L_3\ket{j,m} = n_{-,j,m}^2
    \\

    \\
    \hbar^2 j(j+1) - \hbar^2 m^2 + \hbar^2 m \braket{j,m}{j,m} = n_{-,j,m}^2
    \\

    \\
    \hbar^2 [j(j+1) - m(m-1)] = n_{-,j,m}^2
  \end{array}
\end{equation}

We can write now:

\begin{equation}
  \begin{array}{c}
    L_- \ket{j,m} = \hbar \sqrt{j(j+1) - m(m-1)} \ket{j,m+1}
  \end{array}
\end{equation}

And for $m=-j$ we get 0 again, as we wanted. Knowing $L_+$ and $L_$ we can get the values for all the three components of the angular momentum.

\begin{equation}
  \begin{array}{c}
    L_1 = \frac{L_+ + L_-}{2}
    \\

    \\
    L_2 = \frac{L_+ - L_-}{2i}
  \end{array}
\end{equation}

The components of $\vec{L}$ acting on $\ket{j,m}$ are:



\begin{equation*}
  \label{9.43}
  \begin{array}{l}
    L_1 \ket{j,m} = \frac{\hbar}{2}(\sqrt{j(j+1) - m(m+1)}\ket{j,m+1} + \sqrt{j(j+1) - m(m-1)}\ket{j,m-1})
    \\

    \\
    L_2 \ket{j,m} = \frac{\hbar i}{2}(\sqrt{j(j+1) - m(m+1)}\ket{j,m+1} - \sqrt{j(j+1) - m(m-1)}\ket{j,m-1})
    \\

    \\
    L_3 \ket{j,m} = \hbar m \ket{j,m}
  \end{array}
\end{equation*}

Using the knowledge from chapter 6, if we want to get the excat values for every component of the three operators we can apply \ref{6.16}.


\begin{equation*}
  \begin{array}{l}
    (L_1)_{j_1m_1,j_2,m_2} = \bra{j_1,m_1}L_1\ket{j_2,m_2} = \frac{\hbar}{2}[\sqrt{j_2(j_2+1)-m_2(m_2+1)}\delta_{j_1j_2,m_1m_2+1} + \sqrt{j_2(j_2+1)-m_2(m_2-1)}\delta_{j_1j_2,m_1m_2-1}]
    \\

    \\
    (L_2)_{j_1m_1,j_2,m_2} = \bra{j_1,m_1}L_2\ket{j_2,m_2} = \frac{-\hbar i}{2}[\sqrt{j_2(j_2+1)-m_2(m_2+1)}\delta_{j_1j_2,m_1m_2+1} - \sqrt{j_2(j_2+1)-m_2(m_2-1)}\delta_{j_1j_2,m_1m_2-1}]
    \\

    \\
    (L_3)_{j_1m_1,j_2,m_2} = \bra{j_1,m_1}L_3\ket{j_2,m_2} = \hbar m_2 \delta_{j_1j_2,m_1m_2}
  \end{array}
\end{equation*}

We can see at first sight that $L_3$ has to be a diagonal matrix, while $L_1$ and $L_2$ can only have non-zero values on the secondary diagonals. In the next section we will get the values of the matrix for some j.

\section{Matrix representation for j={1, 1/2, 2}}


The case for j=0 is a trivial case. We are going to start with j=1, where the set of values for m is m={1,0,-1}. We are going to define the matrices as:

\begin{equation}
  L_a =
    \left[\begin{matrix}
      (L_a)_{-1,-1} & (L_a)_{-1,0} & (L_a)_{-1,1}\\
      (L_a)_{0,-1} & (L_a)_{0,0} & (L_a)_{0,1}\\
      (L_a)_{1,-1} & (L_a)_{1,0} & (L_a)_{1,1}
    \end{matrix}\right]
\end{equation}

Where the subindixes of the components represent $m_1$ and $m_2$. We can use the expresions from \ref{9.44} to get the matrix representation of the angular momentum.


\begin{equation}
  L_1 = \frac{\hbar}{\sqrt{2}}
    \left[\begin{matrix}
      0 & 1 & 0\\
      1 & 0 & 1\\
      0 & 1 & 0
    \end{matrix}\right],
  L_2 = \frac{i\hbar}{\sqrt{2}}
    \left[\begin{matrix}
      0 & 1 & 0\\
      -1 & 0 & 1\\
      0 & -1 & 0
    \end{matrix}\right],
  L_3 = \hbar
    \left[\begin{matrix}
      -1 & 0 & 0\\
      0 & 0 & 0\\
      0 & 0 & 1
    \end{matrix}\right]
\end{equation}

We can find the other operators we are interested in just aplying matrix multiplication.

