\setchapterpreamble[u]{\margintoc}
\chapter{The Harmonic Oscillator in 3D}
\labch{intro}

We are going to start from equation \ref{9.115}, that was our Schoringüer Wave Equation in 3D before aplying the potential.

\begin{equation}
\frac{\partial^2 W}{\partial^2 r}+\frac{2(j+1)}{r}\frac{\partial W}{\partial r} + \frac{2m}{\hbar^2}[E-V(r)]W = 0
\end{equation}

The potential is going to be given by the expression:

\begin{equation}
  V = \frac{1}{2} k (x^2+y^2+z^2) = \frac{1}{2} k r^2
\end{equation}

We are going to change our variable.

\begin{equation}
  \begin{array}{c}
    r=bu
    \\

    \\
    W(r=bu) = \chi(u)
  \end{array}
\end{equation}

We are going to substitute the variable in the Schoringüer Wave Equation.

\begin{equation}
  \frac{1}{b^2}\frac{\partial^2\chi}{\partial^2 r}+ \frac{2(j+1)}{b^2 u}\frac{\partial \chi}{\partial u}+\left(\frac{2mE}{\hbar^2}+\frac{2m}{\hbar^2}\frac{1}{2}kb^2u^2\right)\chi = 0
\end{equation}
