\setchapterpreamble[u]{\margintoc}
\chapter{The Hydrogen Atom}
\labch{intro}

This is a very common and well study problem in quantum mechanics. The hydrogen atom is the simplest atom, and it is composed by a proton and an electron. The proton is located at the origin of the coordinate system, and the electron is located at a distance $r$ from the proton. The electron is described by a wave function $\psi(r,\theta,\phi)$, and the potential energy is given by the Coulomb potential. During this chapter we will go through all the theory and compare it with the result from the experiment done in the Modern Physics Lab.


\section{The electric potential}

The electric potential is well known since the 18th century. The potential is given by:

\begin{equation}
  \label{10.1}
  \begin{array}{c}
    V(r) = -\frac{1}{4\pi\epsilon_0}\frac{Ze^2}{r}
  \end{array}
\end{equation}

Where $Z$ is the atomic number of the atom, $e$ is the absolut value of the charge of the electron, and $\epsilon_0$ is the vacuum permittivity. We are also going to define $\hbar$ as the Plank's constant and $m$ as the relative mass in this case, the mass of the electron. All these values are well known and the values get better every year. These values are:

\begin{equation}
  \begin{array}{c}
    e = 1.602176634 \cdot 10^{-19} \, \text{C} \\
    \epsilon_0 = 8.8541878128 \cdot 10^{-12} \, \frac{C^2 s^2}{kg m^2} \\
    m = 9.1093837015 \cdot 10^{-31} \, \text{kg}\\
    \hbar = 1.054571817 \cdot 10^{-34} \, \frac{kg m^2}{s}
  \end{array}
\end{equation}

We are going to look at the wave equation with natural units.

\begin{equation}
  \begin{array}{c}
    r = b u
    \\

    \\
    W_{E,j}(r=bu) = \chi_{E,j}(u)
  \end{array}
\end{equation}

So the wave equation is:

\begin{equation}
  \begin{array}{c}
  \frac{1}{b^2} \frac{d^2\chi}{du^2} + \frac{2(j+1)}{b^2 u}\frac{d \chi}{du} + \left(\frac{2mE}{\hbar^2} + \frac{2m}{\hbar^2}\frac{Ze^2}{4\pi\epsilon_0}\frac{1}{ub}\right)\chi = 0
  \\

  \\
  \frac{d^2\chi}{du^2} + \frac{2(j+1)}{u} \frac{d\chi}{du} + \left(\frac{2mEb^2}{\hbar^2}+\frac{2m}{\hbar^2}\frac{Ze^2 b}{4\pi\epsilon_0}\frac{1}{u}\right)\chi = 0
  \end{array}
\end{equation}

We want to find b so the term that belongs to the potential is equal to 1.

\begin{equation}
  \begin{array}{c}
    b = \frac{2\pi \epsilon_0 \hbar^2}{Z e^2 m} = [m] = \frac{1}{Z} 2.64588603 \cdot 10^{-11} m
  \end{array}
\end{equation}

That number is the natural atomic unit for length. The natural scal, b, becomes smaller with bigger Z.

We can also define the energy in natural units.

\begin{equation}
  \begin{array}{c}
    E = -\frac{\hbar^2}{2mb^2}\alpha
  \end{array}
\end{equation}

Where alpha can be either positive or negative. The wave equation looks like:

\begin{equation}
  \begin{array}{c}
    \frac{d^2\chi}{du^2} + \frac{2(j+1)}{u}\frac{d\chi}{du}-\alpha\chi +\frac{1}{u}\chi= 0
  \end{array}
\end{equation}

When u goes to infinite the equation become:

\begin{equation}
  \begin{array}{c}
    \frac{d^2\chi}{du^2} = \alpha\chi \rightarrow \chi = C_1 e^{-\sqrt{\alpha}u} - C_2 e^{\sqrt{\alpha}u}
  \end{array}
\end{equation}

Since $\chi$ has to go to 0 when $u$ goes to infinite, because of the normalization condition, $C_2$ is going to be 0 and alpha has to be postive, sowe can rewrite this in terms of:

\begin{equation}
  \begin{array}{c}
    \alpha=\beta^2
    \\

    \\
    E = -\frac{Z^2e^4m}{8\pi^2\epsilon_0^2\hbar^2}\beta^2
    \\

    \\
    \chi(u) = e^{-\beta u}R(u)
  \end{array}
\end{equation}

We are going to find the different terms in the wave equation separatly.

\begin{equation}
  \begin{array}{c}
    \frac{d^2\chi}{du^2} = \beta^2 e^{-\beta u} R - 2\beta e^{-\beta u} \frac{dR}{du}+e^{-\beta u} \frac{d^2R}{du^2}
    \\

    \\
    \frac{2(j+1)}{u} \frac{d\chi}{du} = \frac{-2(j+1)}{u} e^{\beta u} R + \frac{2(j+1)}{u} e^{\beta u} \frac{dR}{du}
    \\

    \\
    \left(\frac{1}{u}-\beta^2\right)\chi = \frac{1}{u} e^{\beta u}R -e^{\beta u} R
  \end{array}
\end{equation}

So the wave equation looks like:

\begin{equation}
  u\frac{d^2R}{du^2}+(2(j+1)-2\beta u)\frac{dR}{du} + (1 - 2(j+1)\beta)R = 0
\end{equation}

We can solve this differential equation using the power series method. We are going to assume that the solution is a power series.

\begin{equation}
  \begin{array}{c}
    R(u) = \sum_{k=0}^{\infty} C_k u^k
    \\

    \\
    \frac{dR}{du} = \sum_{k=0}^{\infty} C_{k+1} (k+1) u^{k}
    \\

    \\
    \frac{d^2R}{du^2} = \sum_{k=0}^{\infty} C_{k+1} k(k+1) u^{k-1}
  \end{array}
\end{equation}

We can substitute this into the wave equation, trying to match the indices of all the terms to the same $u^{k}$ and we get:

\begin{equation}
  \begin{array}{c}
    \sum_{k=0}^{\infty} C_{k+1} k (k+1) u^k +
    \\

    \\
    \sum_{k=0}^{\infty} C_{k+1} (k+1) 2(j+1) u^k -
    \\

    \\
    \sum_{k=0}^{\infty} C_{k} 2\beta k u^k +
    \\

    \\
    \sum_{k=0}^{\infty} C_{k} (1-2(j+1)\beta) u^k = 0
    \\

    \\
    \sum_{k=0}^{\infty} u^k\left[C_{k+1}\left[k(k+1)+2(k+1)(j+1)\right]+ \right.
    \\

    \\
    \left. C_k \left[ 1-2(j+1)\beta-2\beta k \right]\right] = 0
    \\

    \\
    C_{k+1} =\frac{2\beta k-1+2\beta(j+1)}{(k+1)(k+2(j+1))}C_k = \frac{2\beta (k+j+1)-1}{(k+1)(k+2(j+1))} C_k
  \end{array}
\end{equation}

The power serie has to be finite because the $R_E,j(u)$ has to be normaliable. This means that for some k=p the coefficient $C_{p+1}$ has to be 0.

\begin{equation}
  \begin{array}{c}
    2\beta (p+j+1) -1 = 0
    \\

    \\
    \beta = \frac{1}{2(p+j+1)} = \frac{1}{2n}
  \end{array}
\end{equation}

Where n is $n=p+j+1$. Because p and j are define as integer numbers from 0 to infinte, n is an integer number, but from 1 to infinite. Now we can define the energy in terms of n.

\begin{equation}
  \begin{array}{c}
    E = -\frac{Z^2 e^4 m}{32\pi^2\epsilon_0^2\hbar^2 n^2} = -2.1798723637575177e-18 \frac{1}{n^2}
  \end{array}
\end{equation}

That is the energy for the eigen-functions:

\begin{equation}
  \begin{array}{c}
    \psi_{n,j,m} = \left(\sum_{k=0}^{n-j-1} C_k u^k \right)e^{-\frac{1}{2n}u}(bu)^j P_j^m(\theta)e^{im\phi}
    \\

    \\
    \psi_{n,j,m} = \left(\sum_{k=0}^{n-j-1} C_k \left(\frac{r}{b}\right)^k \right)e^{-\frac{r}{2nb}}r^j P_j^m(\theta)e^{im\phi}
  \end{array}
\end{equation}

We can plot some of the eigen-functions to see how they look like.

\section{Eigen-functions of the hydrogen atom}

This are some of the solutions from the Hydrogen atom.

For n=1,j=0,m=0:

\begin{equation}
  \psi_{1,0,0} = C_0 e^{-r/2b}
\end{equation}

We can find the normalization constant by using the normalization condition:

\begin{equation}
\begin{array}{c}
  \int_{0}^{2\pi}\int_{0}^{\pi}\int_{0}^{\infty} \psi^*\psi r^2 \sin(\theta) dr d\theta d\phi = 1
  \\

  \\
  \int_{0}^{2\pi}\int_{0}^{\pi}\int_{0}^{\infty} C_0^2 e^{-r/b} r^2 \sin(\theta) dr d\theta d\phi = 1
  \\

  \\
  4 \pi C_0^2 \int_{0}^{\infty} e^{-r/b} r^2 dr = 1
  \\

  \\
  4 \pi C_0^2 (2b^3) = 1
  \\

  \\
  C_0 = \frac{1}{\sqrt{8\pi b^3}}
\end{array}
\end{equation}

The final solution is:

\begin{equation}
  \psi_{1,0,0} = \frac{1}{\sqrt{8\pi b^3}} e^{-r/2b}
\end{equation}


\begin{figure}[H]
  \centering
  \includegraphics{images9/3d_plot_1,0,0.png}
  \caption{Probability distribution (n=1,j=0,m=0)}
\end{figure}

For n=2,j=0,m=0:

\begin{equation}
  \psi_{2,0,0} = \left[C_0-\frac{1}{4}C_0 \frac{r}{b}\right] e^{-r/4b}
\end{equation}

We can find the normalization constant by using the normalization condition:

\begin{equation}
\begin{array}{c}
  \int_{0}^{2\pi}\int_{0}^{\pi}\int_{0}^{\infty} \psi^*\psi r^2 \sin(\theta) dr d\theta d\phi = 1
  \\

  \\
  \int_{0}^{2\pi}\int_{0}^{\pi}\int_{0}^{\infty} C_0^2 \left[C_0-\frac{1}{4}C_0 \frac{r}{b}\right]^2 e^{-r/2b} r^2 \sin(\theta) dr d\theta d\phi = 1
  \\

  \\
  4 \pi C_0^2 \left(\int_{0}^{\infty} e^{-r/2b} r^2 dr-\frac{1}{2b}\int_{0}^{\infty} e^{-r/2b} r^3 dr + \int_{0}^{\infty}\frac{1}{16b^2}e^{-r(2b)}r^4 dr \right) = 1
  \\

  \\
  4 \pi C_0^2 [(2b^3)2-6(2b^3)+6(2b^3)] = 1
  \\

  \\
  C_0 = \frac{1}{\sqrt{64\pi b^3}}
\end{array}
\end{equation}

The final solution is:

\begin{equation}
  \psi_{2,0,0} = \frac{1}{\sqrt{64\pi b^3}} \left[1-\frac{1}{4}\frac{r}{b}\right] e^{-r/4b}
\end{equation}



\begin{figure}[H]
  \centering
  \includegraphics{images9/3d_plot_2,0,0.png}
  \caption{Probability distribution (n=2,j=0,m=0)}
\end{figure}


For n=2,j=1,m=1:

\begin{equation}
  \psi_{2,1,1} = C_0 e^{-r/4b} r \sin\theta e^{i\phi}
\end{equation}

We can find the normalization constant by using the normalization condition:

\begin{equation}
\begin{array}{c}
  \int_{0}^{2\pi}\int_{0}^{\pi}\int_{0}^{\infty} \psi^*\psi r^2 \sin(\theta) dr d\theta d\phi = 1
  \\

  \\
  \int_{0}^{2\pi}\int_{0}^{\pi}\int_{0}^{\infty} C_0^2 e^{-r/2b} r^2 \sin^2\theta r^2 \sin(\theta) dr d\theta d\phi = 1
  \\

  \\
  2 \pi C_0^2\int_{0}^{\pi}\sin^3\theta d\theta \int_{0}^{\infty} e^{-r/b} r^4 dr = 1
  \\

  \\
  2 \pi C_0^2 (\frac{4}{3}) (24(2b)^5) = 1
  \\

  \\
  C_0 = \frac{1}{\sqrt{2^{11}\pi b^5}}
\end{array}
\end{equation}

The final solution is:

\begin{equation}
  \psi_{2,1,1} = \frac{1}{\sqrt{2^{11}\pi b^5}} e^{-r/4b} r \sin\theta e^{i\phi}
\end{equation}

\begin{figure}
  \centering
  \includegraphics{images9/3d_plot_2,1,1.png}
  \caption{Probability distribution (n=2,j=1,m=1)}
\end{figure}

For n=2,j=1,m=0:

\begin{equation}
  \psi_{2,1,0} = C_0 e^{-r/4b} r \cos\theta
\end{equation}

We can find the normalization constant by using the normalization condition:

\begin{equation}
\begin{array}{c}
  \int_{0}^{2\pi}\int_{0}^{\pi}\int_{0}^{\infty} \psi^*\psi r^2 \sin(\theta) dr d\theta d\phi = 1
  \\

  \\
  \int_{0}^{2\pi}\int_{0}^{\pi}\int_{0}^{\infty} C_0^2 e^{-r/2b} r^2 \cos^2\theta r^2 \sin(\theta) dr d\theta d\phi = 1
  \\

  \\
  2 \pi C_0^2\int_{0}^{\pi}\cos^2\theta\sin\theta d\theta \int_{0}^{\infty} e^{-r/b} r^4 dr = 1
  \\

  \\
  2 \pi C_0^2 (\frac{2}{3}) (24(2b)^5) = 1
  \\

  \\
  C_0 = \frac{1}{\sqrt{2^{10}\pi b^5}}
\end{array}
\end{equation}

The final solution is:

\begin{equation}
  \psi_{2,1,0} = \frac{1}{\sqrt{2^{10}\pi b^5}} e^{-r/4b} r \cos\theta
\end{equation}


\begin{figure}
  \centering
  \includegraphics{images9/3d_plot_2,1,0.png}
  \caption{Probability distribution (n=2,j=1,m=0)}
\end{figure}

For n=1,j=1,m=-1:

\begin{equation}
  \psi_{2,1,-1} = C_0 e^{-r/4b} r \sin\theta e^{-i\phi}
\end{equation}

We can find the normalization constant by using the normalization condition:

\begin{equation}
\begin{array}{c}
  \int_{0}^{2\pi}\int_{0}^{\pi}\int_{0}^{\infty} \psi^*\psi r^2 \sin(\theta) dr d\theta d\phi = 1
  \\

  \\
  \int_{0}^{2\pi}\int_{0}^{\pi}\int_{0}^{\infty} C_0^2 e^{-r/2b} r^2 \sin^2\theta r^2 \sin(\theta) dr d\theta d\phi = 1
  \\

  \\
  2 \pi C_0^2\int_{0}^{\pi}\sin^3\theta d\theta \int_{0}^{\infty} e^{-r/b} r^4 dr = 1
  \\

  \\
  2 \pi C_0^2 (\frac{4}{3}) (24(2b)^5) = 1
  \\

  \\
  C_0 = \frac{1}{\sqrt{2^{11}\pi b^5}}
\end{array}
\end{equation}

The final solution is:

\begin{equation}
  \psi_{2,1,-1} = \frac{1}{\sqrt{2^{11}\pi b^5}} e^{-r/4b} r \sin\theta e^{i\phi}
\end{equation}


\begin{figure}
  \centering
  \includegraphics{images9/3d_plot_2,1,-1.png}
  \caption{Probability distribution (n=2,j=1,m=-1)}
\end{figure}


\section{Temperature and Light}

If we look at the plot of  the energy depending on n,we are going to see that the gap between the first energies is bigger than those of the higher energies. To move from one energy level to a higer one we need some temperature. The energy needed to move from the energy $E_i$ to $E_f$ is determined by the factor $KT$, where $K$ is the Boltzmann constant and $T$ is the temperature.

\begin{equation}
  \begin{array}{c}
    \Delta E = E_f - E_i = KT
  \end{array}
\end{equation}

This means that if the temperature is higher we will be able to reach higher energies. However the probability of the particle to be in the lowest energy is always greater or equal than the energy of the particle to be in a higher energy level. This is given by the Boltzmann distribution.

\begin{equation}
  \begin{array}{c}
    P(E_n) \propto e^{-\frac{E_n}{KT}}
  \end{array}
\end{equation}

In the same way we can see that energy can be emitted from the electron when it change from a higher energy to a lower energy state. This energy is going to be emitted in the form of light. The energy of the light is going to be the same as the energy difference between the two energy levels.

\begin{equation}
  \begin{array}{c}
    \Delta E = E_f - E_i = h\omega_{light}
  \end{array}
\end{equation}

\section{Comparison with the experiment}

We are going to look at the lab experiment done by Kevin A. Acosta, partner in this clasroom that was friendly enough to let me his report, because i haven't done the experiment myself.


\begin{marginfigure}
  \centering
  \includegraphics{images9/experiment.jpeg}
  \caption{Experimental setup}
  \label{figure_experiment}
\end{marginfigure}


The experimental setup can be observed in Figure \ref{figure_experiment}. The experiment was done using a Hydrogen Lamp closed to a collimating slit, a diffraction grating and a telescope. The angle of the diffraction grating is taken after a few initial adjustments. Once everything is prepared the telescope is gently moved until the first line is visible, and that angle will be recorded. After some data analysis we can get the total path length between the two beams of light, (only two orders are being used for the experiment). Knowing the total path length one can determined the wavelength of the light. The wavelength is related with the Rydberg constant and the energy levels, (the one from where the electron is coming and the one where the electron is going). The Rydberg constant is given by:

\begin{equation}
\frac{1}{\lambda} = R_H \left(\frac{1}{n_1^2}-\frac{1}{n_2^2}\right)
\end{equation}

This equation can be used in terms of the difference between the energy levels, and is what we are going to use to determined the theoretical Rydberg constant.

\begin{equation}
  R = \frac{4}{3} \frac{E_2-E_1}{c h}
\end{equation}

Where c is the speed of light and h is the Plank's constant. The values $E_2$ and $E_1$ are obtain from our analysis in the previous sections. The theoretical value is:

\begin{equation}
  R = \frac{4}{3} \frac{E_2-E_1}{c h} = 1.0973731 \cdot 10^7 m^{-1}
\end{equation}

Comming back to the experiment, after some analysis of the data we can observed that the $n_1$ we are measuring is actually n=2. This is because only the photons emited from n=3,4,5 and 6 to n=2 have frequencies in the visible spectrum, any other transition will not be appreciate without more sotisficate observational methods. The experimental value of the Rydberg constant in Kevin's experiment is:

\begin{equation}
  R_{exp} = 1.097 \cdot 10^7 \pm 5.656 \cdot 10^{-1} m^{-1}
\end{equation}

This value is very similar to the one obtained using the model we have been working through the whole chapter. So we can say that the theory does explain the experiments, which is our main goal because physics is a experimental science.
